code/experimental/aes/Hacl.Impl.AES_128.Core.fsti
@@ -130,7 +130,8 @@ val xor_state_key1:
   (ensures  (fun h0 _ h1 -> modifies1 st h0 h1 /\
     (
       match m with 
-      |M32 -> seqToTuple (as_seq h1 st) == xor_state_s (seqToTuple (as_seq h0 st)) (seqToTuple (as_seq h0 key))
+      |M32 -> seqToTuple (as_seq h1 st) == xor_state_s (seqToTuple (as_seq h0 st)) (seqToTuple (as_seq h0 key)) /\
+	seqToBlock4 (as_seq h1 st) == Hacl.Spec.AES.xor_block (seqToBlock4 (as_seq h0 st)) (seqToBlock4(as_seq h0 key))
       |MAES -> True
 	     
   )))
